src/specs/alt/option.fst
@@ -1,0 +1,10 @@
+(*--build-config
+--*)
+
+module Tesseract.Specs.Alt.Option
+
+   val get: o: option 'a{is_Some o} -> Tot 'a
+   let get o =
+      match o with
+         | Some a ->
+            a
